Minor changes

ref_impl/src/verifier/experiments/fstar_experiments/project/sequence.fst
@@ -8,3 +8,10 @@ val mapSequence : ('a -> Tot 'b) -> #n:nat -> (sequence 'a n) -> Tot (sequence '
 let rec mapSequence f #n seq = match seq with
 | SNil -> SNil
 | SCons hd tl -> SCons (f hd) (mapSequence f tl)
+
+val zipSequence : #a:Type -> #b:Type -> #n:nat -> sequence a n -> sequence b n -> Tot (sequence (a * b) n)
+let rec zipSequence #a #b #n v1 v2 = match v1 with
+  | SNil -> SNil
+  | SCons a tl1 ->
+    let SCons b tl2 = v2 in
+    SCons (a, b) (zipSequence tl1 tl2)
